\documentclass[12pt, twoside]{article}
\input{../preamble}
\usepackage{float}

\fancyhead[LE]{\thepage}
\fancyhead[RO]{\thepage \\ First and last name: \hspace{2.5cm} \,\\ Section: \hspace{2.5cm} \,}
\fancyhead[LO]{BECA / Dr. Huson / Regents Prep: Graphs\\* 14 November 2024}

\begin{document}

\subsubsection*{3.2 Do Now: Graphing quadratic systems}
\begin{enumerate}
  \item The quadratic of a system of equations is graphed. Add a graph of the linear equation. Mark the intersections as ordered pairs.

  \begin{multicols}{2}
    $y = a(x^2 - 2x - 2)$ \\
    \columnbreak
    $2x-y = 0$
    \end{multicols}
    Find the value of the $a$ coefficient for the second order polynomial. \vspace{2cm}

  \begin{center}
  \begin{tikzpicture}[scale=.635]
    \draw [help lines] (-10,-10) grid (10,10);
    \draw [thick, ->] (-10.2,0) -- (10.4,0) node [below right] {$x$};
    \draw [thick, ->] (0,-10.2)--(0,10.4) node [left] {$y$};
    \draw[thick, <->,smooth, domain=-1.75:3.75] plot (\x, {-2*(\x)^2 + 4*\x + 4});
  \end{tikzpicture}
  \end{center}

\newpage
\item Circle the equations that are an identities.
    \begin{multicols}{2}
      \begin{enumerate}
        \item \(x^2 - y^2 = (x - y)^2\)
        \item \(x^2 + y^2 = x^2 - 2xy + y^2\)
        \item \(x^3 - y^3 = (x - y)(x^2 + xy + y^2)\)
        \item \(x^3 + y^3 = (x + y)(x^2 + xy + y^2)\)
      \end{enumerate}
    \end{multicols}

\item Write a recursive definition of the sequence $a_1 = -2$, $a_2 = 4$, $a_3 = -8$, $a_4 = 16, \ldots$ \vspace{2cm}
    
\item Write down the solutions to the equation $x(2x+3)(x +2)(x - 7) = 0$ \vspace{2cm} 

\item Graphed is $f(x) = x^3+2x^2-5x-6$. Write the function in factored form. 
    \begin{flushright}
    \begin{tikzpicture}[xscale=1, yscale=0.25]
        \draw [thick, ->] (-3.2,0) -- (4,0) node [above] {$x$};
        \draw [thick, ->] (0,-9.2)--(0,10) node [right] {$y$};
        \foreach \x in {-3,...,3} \draw (\x cm,12pt) -- (\x cm,-12pt) node[below] {$\x$};
        \foreach \y in {-8,-6,4,8} \draw (3pt,\y cm) -- (-3pt,\y cm) node[left] {$\y$};
        \draw [thick, <->,smooth,samples=20,domain=-3.3:2.4] plot(\x,{(\x-2)*(\x+1)*(\x+3)});
    \end{tikzpicture}
    \end{flushright}

\item Solve algebraically for $x$: $\displaystyle \frac{1}{x^2} + \frac{1}{2x} = \frac{6}{3x}$ 
\vspace{4cm}


\end{enumerate}
\end{document}